src/Specific/Framework/RawCurveParameters.v
@@ -37,8 +37,10 @@ Record CurveParameters :=
 
     mul_code : option (Z^sz -> Z^sz -> Z^sz);
     square_code : option (Z^sz -> Z^sz);
-    upper_bound_of_exponent
+    upper_bound_of_exponent_tight
     : option (Z -> Z) (* defaults to [fun exp => 2^exp + 2^(exp-3)] for non-montgomery, [fun exp => 2^exp - 1] for montgomery *);
+    upper_bound_of_exponent_loose
+    : option (Z -> Z) (* defaults to [3 * upper_bound_of_exponent_tight] for non-montgomery, [fun exp => 2^exp - 1] for montgomery *);
     allowable_bit_widths
     : option (list nat) (* defaults to [bitwidth :: 2*bitwidth :: nil] *);
     freeze_extra_allowable_bit_widths
@@ -61,7 +63,8 @@ Declare Reduction cbv_RawCurveParameters
             ladderstep
             mul_code
             square_code
-            upper_bound_of_exponent
+            upper_bound_of_exponent_tight
+            upper_bound_of_exponent_loose
             allowable_bit_widths
             freeze_extra_allowable_bit_widths
             modinv_fuel].
