src/Specific/X25519/C32/fesubDisplay.v
@@ -1,0 +1,4 @@
+Require Import Crypto.Specific.X25519.C32.fesub.
+Require Import Crypto.Specific.Framework.IntegrationTestDisplayCommon.
+
+Check display sub.
