src/Specific/X2555/C128/ladderstep.v
@@ -9,11 +9,11 @@ Definition xzladderstep :
   | forall x1 Q Q',
       let xz := xzladderstep x1 Q Q' in
       let eval := B.Positional.Fdecode wt in
-      feW_bounded x1
-      -> feW_bounded (fst Q) /\ feW_bounded (snd Q)
-      -> feW_bounded (fst Q') /\ feW_bounded (snd Q')
-      -> ((feW_bounded (fst (fst xz)) /\ feW_bounded (snd (fst xz)))
-          /\ (feW_bounded (fst (snd xz)) /\ feW_bounded (snd (snd xz))))
+      feW_tight_bounded x1
+      -> feW_tight_bounded (fst Q) /\ feW_tight_bounded (snd Q)
+      -> feW_tight_bounded (fst Q') /\ feW_tight_bounded (snd Q')
+      -> ((feW_tight_bounded (fst (fst xz)) /\ feW_tight_bounded (snd (fst xz)))
+          /\ (feW_tight_bounded (fst (snd xz)) /\ feW_tight_bounded (snd (snd xz))))
          /\ Tuple.map (n:=2) (Tuple.map (n:=2) phiW) xz = FMxzladderstep (m:=m) (eval (proj1_sig a24_sig)) (phiW x1) (Tuple.map (n:=2) phiW Q) (Tuple.map (n:=2) phiW Q') }.
 Proof.
   Set Ltac Profiling.
