src/Specific/solinas32_2e255m2e4m2e1m1/femul.v
@@ -3,8 +3,8 @@ Require Import Crypto.Specific.solinas32_2e255m2e4m2e1m1.Synthesis.
 
 (* TODO : change this to field once field isomorphism happens *)
 Definition mul :
-  { mul : feBW -> feBW -> feBW
-  | forall a b, phiBW (mul a b) = F.mul (phiBW a) (phiBW b) }.
+  { mul : feBW_loose -> feBW_loose -> feBW_tight
+  | forall a b, phiBW_tight (mul a b) = F.mul (phiBW_loose a) (phiBW_loose b) }.
 Proof.
   Set Ltac Profiling.
   Time synthesize_mul ().
