src/Specific/solinas64_2e150m3/fesquare.v
@@ -3,8 +3,8 @@ Require Import Crypto.Specific.solinas64_2e150m3.Synthesis.
 
 (* TODO : change this to field once field isomorphism happens *)
 Definition square :
-  { square : feBW -> feBW
-  | forall a, phiBW (square a) = F.mul (phiBW a) (phiBW a) }.
+  { square : feBW_loose -> feBW_tight
+  | forall a, phiBW_tight (square a) = F.mul (phiBW_loose a) (phiBW_loose a) }.
 Proof.
   Set Ltac Profiling.
   Time synthesize_square ().
